\section{Appendix}
\subsection{Examples}
\subsubsection{Propositional logic to Conjunctive Normal Form}\label{sec:CNF_conversion_Examp}
In the following, we will go through the entire procedure of converting this formula
\begin{equation}\label{eq:CNF_example1}
    \Big(
        p_1 \leftrightarrow (
            p_2 \vee \neg p_3
        )
    \Big) \wedge \Big(
        p_5 \rightarrow (
            p_1 \uparrow p_4
        )
    \Big) \wedge \Big(
        p_4 \oplus p_2
    \Big),
\end{equation}
 to CNF.
\\
For easy reference, we will redeclare the logical equivalence rules from \autoref{sec:CNF}.
\begin{equation}\label{eq:biimplication}
    A \leftrightarrow B \equiv (A \rightarrow  B) \wedge (B \rightarrow A)
\end{equation}
\begin{equation}\label{eq:XOR}
    A \oplus B \equiv \neg (A \rightarrow B) \vee \neg (B \rightarrow A)
\end{equation}
\begin{equation}\label{eq:implication}
    A \rightarrow B \equiv \neg A \vee B
\end{equation}
\begin{equation}\label{eq:NAND}
    A \uparrow B \equiv \neg (A \wedge B)
\end{equation}
\begin{equation}\label{NOR}
    A \downarrow B \equiv \neg (A \vee B)
\end{equation}
Taking it step-by-step, first, we eliminate all boolean operators except for $\neg$, $\vee$ and $\wedge$.
\\
Using \autoref{eq:biimplication} on \autoref{eq:CNF_example1}
\begin{equation}\label{eq:CNF_example2}
    \bigg(
        \Big(
            p_1 \rightarrow (
                p_2 \vee \neg p_3
            )
        \Big) \wedge \Big(
                (
                    p_2 \vee \neg p_3 
                ) \rightarrow p_1 
            \Big)
    \bigg) \wedge \Big(
        p_5 \rightarrow (
            p_1 \uparrow p_4
        )
    \Big) \wedge \Big(
        p_4 \oplus p_2
    \Big).
\end{equation}
Using \autoref{eq:implication} on \autoref{eq:CNF_example2}
\begin{equation}\label{eq:CNF_example3}
    \bigg(
        \Big(
            \neg p_1 \vee (
                p_2 \vee \neg p_3
            )
        \Big) \wedge \Big(
                \neg (
                    p_2 \vee \neg p_3 
                ) \vee p_1 
            \Big)
    \bigg) \wedge \Big(
        \neg p_5 \vee (
            p_1 \uparrow p_4
        )
    \Big) \wedge \Big(
        p_4 \oplus p_2
    \Big).
\end{equation}
Using \autoref{eq:NAND} on on \autoref{eq:CNF_example3}
\begin{equation}\label{eq:CNF_example4}
    \bigg(
        \Big(
            \neg p_1 \vee (
                p_2 \vee \neg p_3
            )
        \Big) \wedge \Big(
                \neg (
                    p_2 \vee \neg p_3 
                ) \vee p_1 
            \Big)
    \bigg) \wedge \Big(
        \neg p_5 \vee \neg (
            p_1 \wedge p_4
        )
    \Big) \wedge \Big(
        p_4 \oplus p_2
    \Big).
\end{equation}
Using \autoref{eq:XOR} on on \autoref{eq:CNF_example4}
\begin{equation}\label{eq:CNF_example5}
    \bigg(
        \Big(
            \neg p_1 \vee (
                p_2 \vee \neg p_3
            )
        \Big) \wedge \Big(
                \neg (
                    p_2 \vee \neg p_3 
                ) \vee p_1 
            \Big)
    \bigg) \wedge \Big(
        \neg p_5 \vee \neg (
            p_1 \wedge p_4
        )
    \Big) \wedge \Big(
        \neg (
            p_4 \rightarrow p_2
        ) \vee \neg (
            p_2 \rightarrow p_4
        )
    \Big).
\end{equation}
Using \autoref{eq:implication} on on \autoref{eq:CNF_example5}
\begin{equation}\label{eq:CNF_example6}
    \bigg(
        \Big(
            \neg p_1 \vee (
                p_2 \vee \neg p_3
            )
        \Big) \wedge \Big(
                \neg (
                    p_2 \vee \neg p_3 
                ) \vee p_1 
            \Big)
    \bigg) \wedge \Big(
        \neg p_5 \vee \neg (
            p_1 \wedge p_4
        )
    \Big) \wedge \Big(
        \neg (
            \neg p_4 \vee p_2
        ) \vee \neg (
            \neg p_2 \vee p_4
        )
    \Big).
\end{equation}
Second, we propagate negations inward
\begin{equation*}
    \bigg(
        \Big(
            \neg p_1 \vee (
                p_2 \vee \neg p_3
            )
        \Big) \wedge \Big(
                (
                    \neg p_2 \wedge \neg \neg p_3 
                ) \vee p_1 
            \Big)
    \bigg) \wedge \Big(
        \neg p_5 \vee (
            \neg p_1 \vee \neg p_4
        )
    \Big) \wedge \Big(
        (
            \neg \neg p_4 \wedge \neg p_2
        ) \vee (
            \neg \neg p_2 \wedge \neg p_4
        )
    \Big).
\end{equation*}
Third, we remove any redundant double negations
\begin{equation}\label{eq:CNF_example7}
    \bigg(
        \Big(
            \neg p_1 \vee (
                p_2 \vee \neg p_3
            )
        \Big) \wedge \Big(
            (
                \neg p_2 \wedge p_3 
            ) \vee p_1 
            \Big)
    \bigg) \wedge \Big(
        \neg p_5 \vee (
            \neg p_1 \vee \neg p_4
        )
    \Big) \wedge \Big(
        (
            p_4 \wedge \neg p_2
        ) \vee (
            p_2 \wedge \neg p_4
        )
    \Big).
\end{equation}
Next, we put \autoref{eq:CNF_example7} in CNF by utilising the distributive property of boolean operators
\begin{gather*}
    \bigg(
        \Big(
            \neg p_1 \vee (
                p_2 \vee \neg p_3
            )
        \Big) \wedge \Big(
            (
                p_1 \vee \neg p_2 
            ) \wedge (
                p_1 \vee p_3
            ) 
            \Big)
    \bigg) \wedge \Big(
        \neg p_5 \vee (
            \neg p_1 \vee \neg p_4
        )
    \Big) \wedge \bigg(
        \Big(
            (
                p_4 \wedge \neg p_2
            ) \vee p_2
        \Big) \vee \Big(
            (
                p_4 \wedge \neg p_2
            ) \vee \neg p_4 
        \Big)
    \bigg)
    \\
    \equiv
    \\
    \bigg(
        \Big(
            \neg p_1 \vee (
                p_2 \vee \neg p_3
            )
        \Big) \wedge \Big(
            (
                p_1 \vee \neg p_2 
            ) \wedge (
                p_1 \vee p_3
            ) 
            \Big)
    \bigg) \wedge \Big(
        \neg p_5 \vee (
            \neg p_1 \vee \neg p_4
        )
    \Big) \wedge
    \\
    \bigg(
        \Big(
            (
                p_2 \vee p_4
            ) \wedge (
                p_2 \vee \neg p_2
            )
        \Big) \wedge \Big(
            (
                p_4 \vee \neg p_4
            ) \wedge (
                \neg p_2 \vee \neg p_4
            )
        \Big)
    \bigg).
\end{gather*}
Finally, we can remove redundant parentheses
\begin{equation*}
    (
        \neg p_1 \vee p_2 \vee \neg p_3
    ) \wedge (
        p_1 \vee \neg p_2 
    ) \wedge (
        p_1 \vee p_3
    ) \wedge (
        \neg p_5 \vee \neg p_1 \vee \neg p_4
    ) \wedge (
        p_2 \vee p_4
    ) \wedge (
        p_2 \vee \neg p_2
    ) \wedge (
        p_4 \vee \neg p_4
    ) \wedge (
        \neg p_2 \vee \neg p_4
    )
\end{equation*}
Thus, we have put \autoref{eq:CNF_example1} into CNF.

\subsubsection{Conjunctive Normal Form to Clausal Form}\label{sec:CNF_to_Clausal_Examp}
Continuing from \autoref{sec:CNF_conversion_Examp}, we will now convert the CNF formula
\begin{equation*}
    (
        \neg p_1 \vee p_2 \vee \neg p_3
    ) \wedge (
        p_1 \vee \neg p_2 
    ) \wedge (
        p_1 \vee p_3
    ) \wedge (
        \neg p_5 \vee \neg p_1 \vee \neg p_4
    ) \wedge (
        p_2 \vee p_4
    ) \wedge (
        p_2 \vee \neg p_2
    ) \wedge (
        p_4 \vee \neg p_4
    ) \wedge (
        \neg p_2 \vee \neg p_4
    ),
\end{equation*}
into clausal form.
\\
We start by removing trivial clauses, such as $p \vee \neg p$
\begin{equation*}
    (
        \neg p_1 \vee p_2 \vee \neg p_3
    ) \wedge (
        p_1 \vee \neg p_2 
    ) \wedge (
        p_1 \vee p_3
    ) \wedge (
        \neg p_5 \vee \neg p_1 \vee \neg p_4
    ) \wedge (
        p_2 \vee p_4
    ) \wedge (
        \neg p_2 \vee \neg p_4
    ).
\end{equation*}
Then, we replace each disjunction with the corresponding set and collect all the sets into a single set of clauses
\begin{equation*}
    \Big\{
        \{
            \neg p_1, p_2, \neg p_3
        \},
        \{
            p_1, \neg p_2
        \},
        \{
            p_1, p_3
        \},
        \{
            \neg p_5, \neg p_1, \neg p_4
        \},
        \{
            p_2, p_4
        \},
        \{
            \neg p_2, \neg p_4
        \}
    \Big\}
\end{equation*}
We have put \autoref{eq:CNF_example1} into CNF and now, ultimately, also into Clausal Form.

\subsubsection{DPLL: Bigger example}\label{sec:DPLL_Bigger_Example}
In the following we show the DPLL algorithm on the formula \autoref{eq:SAT_example2}.
\begin{figure}[H]
    \centering
    \begin{subfigure}[t]{0.48\textwidth}
        \centering
        \includegraphics[width=\textwidth]{figures/Constraint-Programming/DPLL-Example2/1.png}
        \subcaption*{Step 0: Initially, no literals has been assigned any values.}
    \end{subfigure}
    \hfill
    \begin{subfigure}[t]{0.48\textwidth}
        \centering
        \includegraphics[width=\textwidth]{figures/Constraint-Programming/DPLL-Example2/2.png}
        \subcaption*{Step 1: We start by assigning \texttt{False} to \(p_1\) at random.}
    \end{subfigure}
\end{figure}

\begin{figure}[H]
    \centering
    \begin{subfigure}[t]{0.48\textwidth}
        \centering
        \includegraphics[width=\textwidth]{figures/Constraint-Programming/DPLL-Example2/3.png}
        \subcaption*{Step 2: Then we assign \texttt{False} to \(p_2\) at random.}
    \end{subfigure}
    \hfill
    \begin{subfigure}[t]{0.48\textwidth}
        \centering
        \includegraphics[width=\textwidth]{figures/Constraint-Programming/DPLL-Example2/4.png}
        \subcaption*{Step 3: Thirdly, we assign \texttt{False} to \(p_3\). However, Unit Propagation on clause \(2\) and \(3\) yields to a conflicting assignment.}
    \end{subfigure}
\end{figure}

\begin{figure}[H]
    \centering
    \begin{subfigure}[t]{0.48\textwidth}
        \centering
        \includegraphics[width=\textwidth]{figures/Constraint-Programming/DPLL-Example2/5.png}
        \subcaption*{Step 4: We backtrack and assign \texttt{True} to \(p_3\). This in turn, also yields a conlict from clause \(4\) and \(5\).}
    \end{subfigure}
    \hfill
    \begin{subfigure}[t]{0.48\textwidth}
        \centering
        \includegraphics[width=\textwidth]{figures/Constraint-Programming/DPLL-Example2/6.png}
        \subcaption*{Step 5: Then we backtrack again, assigning \texttt{True} to \(p_2\).}
    \end{subfigure}
\end{figure}

\begin{figure}[H]
    \centering
    \begin{subfigure}[t]{0.48\textwidth}
        \centering
        \includegraphics[width=\textwidth]{figures/Constraint-Programming/DPLL-Example2/7.png}
        \subcaption*{Step 6: We now assign \texttt{False} to \(p_3\) at random. However, once more this leads to a conlfict from clause \(2\) and \(3\).}
    \end{subfigure}
    \hfill
    \begin{subfigure}[t]{0.48\textwidth}
        \centering
        \includegraphics[width=\textwidth]{figures/Constraint-Programming/DPLL-Example2/8.png}
        \subcaption*{Step 7: We backtrack on \(p_3\), assigning it \texttt{True} instead, but this leads to the same prior conlfict on Clause \(4\) and \(5\).}
    \end{subfigure}
\end{figure}

\begin{figure}[H]
    \centering
    \begin{subfigure}[t]{0.48\textwidth}
        \centering
        \includegraphics[width=\textwidth]{figures/Constraint-Programming/DPLL-Example2/9.png}
        \subcaption*{Step 8: We backtrack and assign \texttt{True} to \(p_1\).}
    \end{subfigure}
    \hfill
    \begin{subfigure}[t]{0.48\textwidth}
        \centering
        \includegraphics[width=\textwidth]{figures/Constraint-Programming/DPLL-Example2/10.png}
        \subcaption*{Step 9: Then we try to assign \texttt{False} to \(p_2\), but this now leads to a conlict from clause \(1\) and \(7\).}
    \end{subfigure}
\end{figure}

\begin{figure}[H]
    \centering
    \begin{subfigure}[t]{0.48\textwidth}
        \centering
        \includegraphics[width=\textwidth]{figures/Constraint-Programming/DPLL-Example2/11.png}
        \subcaption*{Step 10: We backtrack and assign \texttt{True} to \(p_2\).}
    \end{subfigure}
    \hfill
    \begin{subfigure}[t]{0.48\textwidth}
        \centering
        \includegraphics[width=\textwidth]{figures/Constraint-Programming/DPLL-Example2/12.png}
        \subcaption*{Step 11: Then we have Unit Propagation from clause \(8\) and we assign \texttt{True} to \(p_3\).}
    \end{subfigure}
\end{figure}

\begin{figure}[H]
    \centering
    \begin{subfigure}[t]{0.48\textwidth}
        \centering
        \includegraphics[width=\textwidth]{figures/Constraint-Programming/DPLL-Example2/13.png}
        \subcaption*{Step 16: Finally, our last assignment \(p_4 =\) \texttt{True} is from Unit Propagation by clause \(6\) and yields the satisfying assignment:
        \\
        \(\mathcal{A} = \{p_1 = \text{\texttt{True}}, p_2 = \text{\texttt{True}}, p_3 = \text{\texttt{True}}, p_4 = \text{\texttt{True}}\}\).}
    \end{subfigure}
\end{figure}


\subsection{Figures}
\begin{figure}[H]
    \centering
    \includegraphics[width=0.8\textwidth]{figures/Danske_Regioner__Sundhedsv√¶senets_digitaliseringsrejse.png}
    \caption{The Danish healthcare sector's road to digitalisation}
    \medskip
    \small
    \raggedright
    The Danish healthcare sector's road to digitalisation, as presented by "Danske Regioner"\cite{Den-Reg-digitalisation}.
    \label{fig:healthcare_digitalisation}
\end{figure}

\begin{figure}[H]
    \centering
    \includegraphics[width=0.75\textwidth]{figures/Questionnaire_for_healthcare_sector.png}
    \caption{Questionnaire for healthcare personnel}
    \medskip
    \small
    \raggedright
    Questionnaire sent to Danish hospitals, in the pursuit of reaching out to healthcare personnel.
    \\
    \textbf{Translated from Danish:}
    \\
    \textbf{Title}: "Engineering project in the healthcare sector"
    \\
    \textbf{Introduction}: "Hello, my name is Felix, I am studying to become an engineer with a focus on Artificial intelligence at DTU. At the moment I am looking for a concrete problem for my master's thesis, and I was hoping to be able to work on a project, which combines technology with healthcare, in an attempt to make a real difference. In that pursuit, I wanted to ask whether you can spare a momemnt to answer this questionnaire." 
    \\
    \textbf{Question 1}: "What is the biggest and most frequent problem in your daily life as a healthcare professional?"
    \\
    \textbf{Question 2}: "What do you think is the biggest and most frequent problem in the daily life of your patients?"
    \\
    \textbf{Question 3}: "Please write your email and name, if I may contact you with follow-up questions."
    \\
    \textbf{Question 4}: "Name (not mandatory)"
    \\
    \textbf{Question 5}: "Email (not mandatory)"
    \label{fig:questionnaire_healthcare_personnel}
\end{figure}